container/coq/revising/Layer12/Spec_drf.v
@@ -41,6 +41,8 @@ Section Layer12_Spec.
     when st_2 == ((spinlock_release_spec (mkPtr "vmid_lock" 0) st_1));
     (Some st_2).
 
+
+
   Fixpoint total_root_rtt_refcount_loop295 (_N_: nat) (__break__: bool) (v_0: Ptr) (v__011: Z) (v__0_lcssa: Z) (v_indvars_iv: Z) (v_wide_trip_count: Z) (st: RData) : (option (bool * Ptr * Z * Z * Z * Z * RData)) :=
     match (_N_) with
     | O => (Some (__break__, v_0, v__011, v__0_lcssa, v_indvars_iv, v_wide_trip_count, st))
